examples/nsl_pk/DY.Example.NSL.Invariants.fst
@@ -1,0 +1,88 @@
+module DY.Example.NSL.Invariants
+
+open Comparse
+open DY.Core
+open DY.Lib
+open DY.Example.NSL.Protocol.Total.Proof
+open DY.Example.NSL.Protocol.Stateful
+open DY.Example.NSL.Protocol.Stateful.Proof
+
+#set-options "--fuel 0 --ifuel 0"
+
+/// Crypto Usages
+
+instance nsl_crypto_usages: crypto_usages = default_crypto_usages
+
+/// List of all local pkenc predicates
+
+let all_pkenc_tag_and_preds = [
+  nsl_tag_and_pkenc_pred;
+]
+
+let nsl_crypto_predicates: crypto_predicates nsl_crypto_usages = {
+  default_crypto_predicates nsl_crypto_usages with
+  pkenc_pred = mk_pkenc_predicate all_pkenc_tag_and_preds
+}
+
+/// Crypto Invariants
+
+instance nsl_crypto_invariants: crypto_invariants = {
+  usages = nsl_crypto_usages;
+  preds = nsl_crypto_predicates;
+}
+
+// fuel 1 is a workaround for FStarLang/FStar#3360
+#push-options "--fuel 1"
+val nsl_crypto_invariants_has_nsl_crypto_invariants:
+  unit ->
+  Lemma (has_nsl_crypto_invariants #nsl_crypto_invariants)
+let nsl_crypto_invariants_has_nsl_crypto_invariants () =
+  assert_norm(List.Tot.no_repeats_p (List.Tot.map fst all_pkenc_tag_and_preds));
+  mk_pkenc_predicate_correct nsl_crypto_invariants all_pkenc_tag_and_preds;
+  norm_spec [delta_only [`%all_pkenc_tag_and_preds; `%for_allP]; iota; zeta] (for_allP (has_pkenc_predicate nsl_crypto_invariants) all_pkenc_tag_and_preds)
+#pop-options
+
+/// List of all local state predicates.
+
+let all_state_tag_and_preds = [
+  pki_tag_and_invariant;
+  private_keys_tag_and_invariant;
+  (local_state_nsl_session.tag, local_state_predicate_to_local_bytes_state_predicate state_predicate_nsl);
+]
+
+/// List of all local event predicates.
+
+let all_event_tag_and_preds = [
+  (event_nsl_event.tag, compile_event_pred event_predicate_nsl)
+]
+
+/// Trace Invariant
+
+let nsl_trace_invariants: trace_invariants nsl_crypto_invariants = {
+  state_pred = mk_state_pred nsl_crypto_invariants all_state_tag_and_preds;
+  event_pred = mk_event_pred all_event_tag_and_preds;
+}
+
+/// Protocol Invariants
+
+instance nsl_protocol_invariants: protocol_invariants = {
+  crypto_invs = nsl_crypto_invariants;
+  trace_invs = nsl_trace_invariants;
+}
+
+// fuel 1 is a workaround for FStarLang/FStar#3360
+#push-options "--fuel 1"
+val nsl_protocol_invariants_has_nsl_invariants:
+  unit ->
+  Lemma (has_nsl_invariants #nsl_protocol_invariants)
+let nsl_protocol_invariants_has_nsl_invariants () =
+  nsl_crypto_invariants_has_nsl_crypto_invariants ();
+
+  assert_norm(List.Tot.no_repeats_p (List.Tot.map fst (all_state_tag_and_preds)));
+  mk_state_pred_correct nsl_protocol_invariants all_state_tag_and_preds;
+  norm_spec [delta_only [`%all_state_tag_and_preds; `%for_allP]; iota; zeta] (for_allP (has_local_bytes_state_predicate nsl_protocol_invariants) all_state_tag_and_preds);
+
+  assert_norm(List.Tot.no_repeats_p (List.Tot.map fst (all_event_tag_and_preds)));
+  mk_event_pred_correct nsl_protocol_invariants all_event_tag_and_preds;
+  norm_spec [delta_only [`%all_event_tag_and_preds; `%for_allP]; iota; zeta] (for_allP (has_compiled_event_pred nsl_protocol_invariants) all_event_tag_and_preds)
+#pop-options
