examples/nsl_pk/DY.Example.NSL.SecurityProperties.fst
@@ -22,41 +22,46 @@ open DY.Example.NSL.Protocol.Stateful.Proof
 /// unless the attacker corrupted Alice or Bob.
 
 val initiator_authentication:
+  {|protocol_invariants|} ->
   tr:trace -> i:timestamp ->
   alice:principal -> bob:principal -> n_a:bytes -> n_b:bytes ->
   Lemma
   (requires
     event_triggered_at tr i bob (Respond2 alice bob n_a n_b) /\
-    trace_invariant tr
+    trace_invariant tr /\
+    has_nsl_invariants
   )
   (ensures
     is_corrupt tr (principal_label alice) \/ is_corrupt tr (principal_label bob) \/
     event_triggered (prefix tr i) alice (Initiate2 alice bob n_a n_b)
   )
-let initiator_authentication tr i alice bob n_a n_b = ()
+let initiator_authentication #invs tr i alice bob n_a n_b = ()
 
 /// If Alice thinks she talks with Bob,
 /// then Bob thinks he talk to Alice (with the same nonces),
 /// unless the attacker corrupted Alice or Bob.
 
 val responder_authentication:
+  {|protocol_invariants|} ->
   tr:trace -> i:timestamp ->
   alice:principal -> bob:principal -> n_a:bytes -> n_b:bytes ->
   Lemma
   (requires
     event_triggered_at tr i alice (Initiate2 alice bob n_a n_b) /\
-    trace_invariant tr
+    trace_invariant tr /\
+    has_nsl_invariants
   )
   (ensures
     is_corrupt tr (principal_label alice) \/ is_corrupt tr (principal_label bob) \/
     event_triggered (prefix tr i) bob (Respond1 alice bob n_a n_b)
   )
-let responder_authentication tr i alice bob n_a n_b = ()
+let responder_authentication #invs tr i alice bob n_a n_b = ()
 
 /// The nonce n_a is unknown to the attacker,
 /// unless the attacker corrupted Alice or Bob.
 
 val n_a_secrecy:
+  {|protocol_invariants|} ->
   tr:trace -> alice:principal -> bob:principal -> n_a:bytes ->
   Lemma
   (requires
@@ -65,16 +70,18 @@ val n_a_secrecy:
       (exists sess_id. state_was_set tr alice sess_id (InitiatorSentMsg1 bob n_a)) \/
       (exists sess_id n_b. state_was_set tr alice sess_id (InitiatorSentMsg3 bob n_a n_b)) \/
       (exists sess_id n_b. state_was_set tr bob sess_id (ResponderReceivedMsg3 alice n_a n_b))
-    )
+    ) /\
+    has_nsl_invariants
   )
   (ensures is_corrupt tr (principal_label alice) \/ is_corrupt tr (principal_label bob))
-let n_a_secrecy tr alice bob n_a =
+let n_a_secrecy #invs tr alice bob n_a =
   attacker_only_knows_publishable_values tr n_a
 
 /// The nonce n_b is unknown to the attacker,
 /// unless the attacker corrupted Alice or Bob.
 
 val n_b_secrecy:
+  {|protocol_invariants|} ->
   tr:trace -> alice:principal -> bob:principal -> n_b:bytes ->
   Lemma
   (requires
@@ -83,8 +90,9 @@ val n_b_secrecy:
       (exists sess_id n_a. state_was_set tr bob sess_id (ResponderSentMsg2 alice n_a n_b)) \/
       (exists sess_id n_a. state_was_set tr bob sess_id (ResponderReceivedMsg3 alice n_a n_b)) \/
       (exists sess_id n_a. state_was_set tr alice sess_id (InitiatorSentMsg3 bob n_a n_b))
-    )
+    ) /\
+    has_nsl_invariants
   )
   (ensures is_corrupt tr (principal_label alice) \/ is_corrupt tr (principal_label bob))
-let n_b_secrecy tr alice bob n_b =
+let n_b_secrecy #invs tr alice bob n_b =
   attacker_only_knows_publishable_values tr n_b
